



## Fol Exercise problems for practise

1 message

Tarachand Amgoth <tarachand@iitism.ac.in>  
To: BIJAY VISHWAKARMA <25et0047@iitism.ac.in>

Tue, Nov 11, 2025 at 11:41 AM

### FOL-Based Equivalence Formulas

1. Show that  $\forall x(P(x) \vee Q(x)) \equiv (\forall xP(x)) \vee (\forall xQ(x))$ .
2. Prove  $\neg(\exists xP(x)) \equiv \forall x\neg P(x)$ .
3. Simplify  $\forall x(\neg P(x) \vee Q(x)) \equiv \forall x(P(x) \Rightarrow Q(x))$ .
4. Prove  $(\forall xP(x)) \vee Q \equiv \forall x(P(x) \vee Q)$ .

### Modus Ponens in FOL

5. Given  $\forall x(P(x) \Rightarrow Q(x))$  and  $P(a)$ , derive  $Q(a)$ .
6. Prove  $(\forall x(R(x) \Rightarrow S(x))) \wedge R(c) \Rightarrow S(c)$  using Modus Ponens.
7. If  $\forall x(P(x) \Rightarrow Q(x)) \wedge \exists yP(y)$ , prove  $\exists yQ(y)$ .
8. Given  $\forall x(A(x) \wedge B(x) \Rightarrow C(x))$  and  $A(a) \wedge B(a)$ , derive  $C(a)$ .
9. Prove  $(\forall x(L(x) \vee M(x))) \wedge \neg M(c) \Rightarrow L(c)$ .

### And Eliminations in FOL

10. From  $\forall x(P(x) \wedge Q(x))$ , derive  $\forall xP(x)$ .
11. Prove  $(\forall x(R(x) \wedge S(x))) \Rightarrow (\forall xR(x))$ .
12. Show  $(\exists x(A(x) \wedge B(x))) \Rightarrow (\exists xA(x)) \wedge (\exists xB(x))$ .

### Forward Chaining in FOL

13. In a knowledge base  $\forall x(P(x) \Rightarrow Q(x))$ ,  $Q(c) \Rightarrow R(c)$ , and  $P(c)$ , derive  $R(c)$ .
14. Given  $\forall x(A(x) \Rightarrow B(x))$ ,  $B(c) \Rightarrow C(c)$ , and  $A(c)$ , prove  $C(c)$ .
15. Use forward chaining to derive  $Q(c)$  from  $P(c) \Rightarrow Q(c)$  and  $P(c)$ .
16. In a rule-based system with  $\forall x(P(x) \Rightarrow (Q(x) \wedge R(x)))$  and  $P(a)$ , derive  $Q(a)$  and  $R(a)$ .
17. Prove  $\forall x(A(x) \Rightarrow B(x))$ ,  $A(c) \Rightarrow B(c)$  using forward chaining.

### Backward Chaining in FOL

18. Prove  $\forall x(P(x) \Rightarrow Q(x))$ ,  $Q(c)$  using backward chaining from  $P(c)$ .
19. Verify  $S(c)$  from  $\forall x(R(x) \Rightarrow S(x))$ ,  $R(c)$ .
20. Use backward chaining to derive  $Q(a)$  from  $Q(x) \Rightarrow R(x)$  and  $R(a)$ .
21. Prove  $(\forall x(A(x) \Rightarrow B(x))) \wedge B(c) \Rightarrow A(c)$ .
22. Verify  $C(c)$  using backward chaining in  $(\forall x(A(x) \Rightarrow C(x))) \wedge A(c)$ .

### Resolution in FOL

23. Resolve  $P(a) \vee Q(a)$  and  $\neg Q(a) \vee R(a)$  to derive  $P(a) \vee R(a)$ .
24. Prove  $Q(c)$  from  $\forall x(P(x) \vee Q(x))$ ,  $\neg P(c)$ .
25. Derive  $R(x)$  from  $\forall x(\neg Q(x) \vee R(x))$ ,  $Q(c)$ .
26. Resolve  $(\forall x(\neg A(x) \vee B(x)))$  and  $\neg B(a)$  to derive  $\neg A(a)$ .
27. Prove  $Q(b) \vee R(b)$  from  $P(a) \vee Q(a)$ ,  $\neg P(a) \vee R(a)$ ,  $Q(a)$ .

### Mixed and Advanced Problems

28. Convert  $\forall x(P(x) \wedge Q(x)) \vee R(x)$  to Skolemized form.
29. Simplify  $\exists x(A(x) \vee \neg A(x))$  using equivalence rules.
30. Use forward chaining to derive conclusions from  $\forall x(P(x) \Rightarrow Q(x))$ ,  $Q(x) \Rightarrow R(x)$ ,  $P(a)$ .
31. Use backward chaining to verify  $T(c) \wedge T(c)$  in a system  $T(x) \Rightarrow (A(x) \vee B(x))$ ,  $\neg A(c)$ .
32. Resolve  $(\neg P(x) \vee Q(x)) \wedge (\neg Q(a) \vee R(a))$  to derive  $R(a) \vee \neg P(a)$ .

33. Show  $\forall x(\neg P(x) \vee \neg Q(x)) \equiv \neg \exists x(P(x) \wedge Q(x))$ .  
 34. Prove  $\forall x(P(x) \Rightarrow Q(x)), P(c) \Rightarrow Q(c)$ .  
 35. Simplify  $\neg(\forall xA(x)) \vee (\exists yB(y))$ .  
 36. Use forward chaining to derive  $C(a)$  from  $A(a) \Rightarrow B(a), B(a) \Rightarrow C(a)$ .  
 37. Prove  $R(a)$  using resolution with  $\forall x(P(x) \vee R(x)), \neg P(a)$ .

### Advanced Mixed Problems

38. Resolve  $(\forall x(A(x) \vee B(x))) \wedge (\neg A(c))$  to derive  $B(c)$ .  
 39. Use backward chaining to verify  $S(x)$  from  $A(x) \Rightarrow S(x), A(c)$ .  
 40. Prove  $\neg \exists x(\neg P(x)) \equiv \forall x(P(x))$ .  
 41. Derive  $Q(c) \vee R(c)$  from  $\neg P(c) \vee Q(c), P(c) \vee R(c)$ .  
 42. Simplify  $\forall x(A(x) \vee \neg B(x)) \wedge (\forall yB(y))$ .  
 43. Resolve  $(\forall x(P(x) \vee Q(x)))$  and  $\neg Q(a)$  to derive  $P(a)$ .  
 44. Prove  $(\forall x(R(x) \Rightarrow S(x))) \wedge R(c) \Rightarrow S(c)$ .  
 45. Use forward chaining to derive  $C(a)$  from  $A(a) \Rightarrow B(a), B(a) \Rightarrow C(a)$ .  
 46. Prove  $\forall x(A(x) \wedge B(x)) \Rightarrow \forall xA(x) \wedge \forall xB(x)$ .  
 47. Convert to CNF:  $\forall x(P(x) \vee Q(x)) \Rightarrow R(x)$ . Hint: Rewrite the implication, eliminate universal quantifier, and distribute disjunction.  
 48. Convert to CNF:  $\neg(\exists x(P(x) \wedge Q(x))) \vee R(a)$ . : Use De Morgan's laws and convert the existential quantifier to universal.  
 49. Convert to CNF:  $\forall x(\neg P(x) \vee (Q(x) \Rightarrow R(x)))$ . Hint: Replace the implication and distribute disjunction over conjunction.  
 50. Convert to CNF:  $(\forall xP(x)) \wedge (\exists yQ(y) \vee R(c))$ . Hint: Skolemize the existential quantifier and standardize variables.  
 51. Convert to CNF:  $\forall x(\neg Q(x) \vee \exists yR(x,y))$ . Hint: Skolemize the existential quantifier and distribute logical operators.  
 52. Convert to CNF:  $(\exists xP(x)) \Rightarrow \forall y(Q(y) \vee R(y))$ . Hint: Replace implication, Skolemize, and standardize variables.  
 53. Convert to CNF:  $\neg(\forall x(P(x) \Rightarrow Q(x)))$ . Hint: Eliminate negation and implication, then apply standard CNF conversion steps.  
 54. Convert to CNF:  $\forall x \forall y((P(x) \vee Q(y)) \Rightarrow R(x,y))$ . Hint: Replace implication, Skolemize if necessary, and distribute.  
 55. Convert to CNF:  $\exists x(\forall y(P(x,y) \vee Q(x)) \Rightarrow R(x))$ . Hint: Carefully Skolemize and distribute disjunctions.  
 56. Convert to CNF:  $\forall x \exists y(\neg P(x) \vee Q(y))$ . Hint: Skolemize the existential quantifier and simplify using logical equivalences.

### Unification Problems

57. Unify  $P(A,x)$  and  $P(y,B)$ . Hint: Find substitutions for  $x$  and  $y$ .  
 58. Determine if  $Q(f(A),B,z)$  and  $Q(x,B,g(y))$  can be unified. If yes, find the unifier. Hint: Match function symbols and variables.  
 59. Unify  $P(A,f(x))$  and  $P(A,f(B))$ . Hint: Focus on the arguments of the function.  
 60. Unify  $R(x,g(A))$  and  $R(f(y),g(z))$ . Hint: Consider nested terms carefully.  
 61. Determine if  $S(x,A,y)S(x,A,y)$  and  $S(g(B),A,g(z))S(g(B),A,g(z))$  can be unified. Hint: Compare  $xx$  and  $g(B)g(B)$ ,  $yy$  and  $g(z)g(z)$ .  
 62. Unify  $Q(x,y,z)$  and  $Q(A,f(B),g(C))$ . Hint: Derive substitutions for  $x,y$ , and  $z$ .  
 63. Determine if  $P(f(A,B),x)$  and  $P(f(y,z),g(A))$  can be unified. Hint: Focus on matching arguments of the function  $f$ .  
 64. Unify  $R(A,g(x))$  and  $R(y,g(B))$ . Hint: Identify substitutions for  $x$  and  $y$ .  
 65. Can  $P(f(x), g(A))$  and  $P(f(A),g(y))$  be unified? Find the substitution if possible. Hint: Ensure consistent substitutions.  
 66. Determine if  $S(f(x,A),B)$  and  $S(f(y,z),w)$  can be unified. Hint: Resolve nested terms  $f(x,A)$  and  $f(y,z)$ .

### Lifting Problems

67. Apply the lifting principle to prove  $\exists xP(x) \Rightarrow P(A)$ . Hint: Instantiate  $x$  with a constant.

68. Demonstrate lifting by generalizing  $P(A) \vee P(B)$  to  $\forall x P(x)$ . Hint: Show the relationship between instances and universal quantification.
69. Use lifting to prove  $\forall x(P(x) \vee Q(x)) \Rightarrow P(A) \vee Q(A)$ . Hint: Substitute  $x$  with a constant and derive the conclusion.
70. Show that  $\forall x(P(x) \wedge Q(x)) \Rightarrow P(y) \wedge Q(y)$  using lifting. Hint: Replace  $x$  with  $y$ .
71. Apply lifting to derive  $\exists y(P(y) \vee Q(y))$  from  $P(A) \vee Q(A)$ . Hint: Introduce an existential quantifier over instances.
72. Prove  $\exists x(P(x) \wedge Q(x)) \Rightarrow P(A) \wedge Q(A)$  using lifting. Hint: Instantiate  $x$  with  $A$ .
73. Use lifting to transform  $P(A) \wedge P(B)$  into  $\forall x P(x)$ . Hint: Generalize from specific instances.
74. Apply lifting to validate  $\forall x(P(x) \vee Q(x)) \Rightarrow \exists y(P(y) \vee Q(y))$ . Hint: Use a general-to-specific reasoning.
75. Show that  $\forall x(P(x) \wedge R(x)) \Rightarrow R(y)$  using lifting. Hint: Replace  $x$  with  $y$ .
76. Demonstrate lifting for  $\exists x P(x) \vee \exists y Q(y) \Rightarrow \exists z(P(z) \vee Q(z))$ . Hint: Use existential generalization.

Thanks & Regards

**Prof. Tarachand Amgoth**  
Associate Professor,  
Computer Science & Engineering,  
Indian Institute of Technology, Dhanbad  
Webpage: [people.iitism.ac.in/~tarachand/](http://people.iitism.ac.in/~tarachand/)